added various things in SetUtil; changed notations; + some renamings

Util/Set/SetUtil.v
@@ -4,75 +4,377 @@ See the COPYRIGHTS and LICENSE files.
 
 - Frederic Blanqui, 2009-06-26
 
-Infinite sets
+Type for representing potentially infinite sets of elements of some type.
 *)
 
 Set Implicit Arguments.
 
-Require Import LogicUtil RelUtil Morphisms Basics.
+Require Import RelUtil LogicUtil Basics Morphisms Setoid FunUtil
+  ListUtil NatUtil ClassicUtil.
 
-Section defs.
+(****************************************************************************)
+(** We assume given a type A for elements. *)
 
-  Variable X : Type.
+Section S.
 
-  Definition set := X -> Prop.
+  Context {A : Type}.
 
-  Definition incl := pointwise_relation X impl.
+  Notation eq_dec_type := (forall x y : A, {x=y}+{~x=y}).
 
-  Definition equiv := pointwise_relation X iff.
+(****************************************************************************)
+(** Type of sets of elements of [A]. *)
+
+  Definition set := A -> Prop.
+
+(****************************************************************************)
+(** Definitions. *)
+
+  Definition mem a (P : set) := P a.
+
+  (*Definition subset (P Q : set) := forall x, mem x P -> mem x Q.*)
+  Definition subset : relation set := pointwise_relation A impl.
+
+  Infix "[<=]" := subset (at level 70).
+
+  (*Definition equiv (P Q : set) := forall x, mem x P <-> mem x Q.*)
+  Definition equiv : relation set := pointwise_relation A iff.
+
+  Infix "[=]" := equiv (at level 70).
+
+  Definition strict_subset P Q := P [<=] Q /\ ~Q [<=] P.
+
+  Infix "[<]" := strict_subset (at level 70).
 
   Definition empty : set := fun _ => False.
 
-  Definition union (A B : set) : set := fun x => A x \/ B x.
+  Definition all : set := fun _ => True.
 
-  Definition singleton x0 : set := fun x => x = x0.
+  Definition add a (P : set) : set := fun x => x = a \/ mem x P.
 
-  Definition add x0 A := union (singleton x0) A.
+  Definition singleton a := add a empty.
 
-End defs.
+  Definition union (P Q : set) : set := fun x => mem x P \/ mem x Q.
 
-Arguments incl {X} A B.
-Arguments equiv {X} A B.
-Arguments empty {X} _.
+  Definition rem a (P : set) : set := fun x => x <> a /\ mem x P.
 
-Infix "[= " := incl (at level 70).
+  Definition diff (P Q : set) : set := fun x => mem x P /\ ~mem x Q.
+
+  Definition of_list l : set := fun x => In x l.
+
+  Ltac stac := intro; unfold add, rem, diff, union, of_list, mem; simpl; tauto.
+
+(****************************************************************************)
+(** Properties of inclusion. *)
+
+  Global Instance subset_PreOrder : PreOrder subset.
+
+  Proof. fo. Qed.
+
+(****************************************************************************)
+(** Properties of equality. *)
+
+  Lemma equiv_subset2 P Q : P [=] Q <-> P [<=] Q /\ Q [<=] P.
+
+  Proof. fo. Qed.
+
+  Global Instance equiv_Equivalence : Equivalence equiv.
+
+  Proof. fo. Qed.
+
+  Global Instance subset_equiv : Proper (equiv ==> equiv ==> impl) subset.
+
+  Proof. fo. Qed.
+
+  Lemma equiv_inter_transp : equiv == inter_transp subset.
+
+  Proof. fo. Qed.
+
+  Lemma equiv_elim P Q : P [=] Q <-> P [<=] Q /\ Q [<=] P.
+
+  Proof. fo. Qed.
+
+(****************************************************************************)
+(** Properties of [mem]. *)
+
+  Global Instance mem_subset : Proper (eq ==> subset ==> impl) mem.
+
+  Proof. intros x y xy P Q PQ. subst. fo. Qed.
+
+  Global Instance mem_equiv_impl : Proper (eq ==> equiv ==> impl) mem.
+
+  Proof. intros x y xy P Q PQ. subst. fo. Qed.
+
+  Global Instance mem_equiv : Proper (eq ==> equiv ==> iff) mem.
+
+  Proof. intros x y xy P Q PQ. subst. fo. Qed.
+
+(****************************************************************************)
+(** Properties of strict inclusion. *)
+
+  Global Instance strict_subset_incl_subset : subrelation strict_subset subset.
+
+  Proof. intros X Y [XY nYX]. hyp. Qed.
+
+  Global Instance strict_subset_Transitive : Transitive strict_subset.
+
+  Proof. intros X Y Z [XY nYX] [YZ nZY]. split. trans Y; hyp. fo. Qed.
+
+  Global Instance strict_subset_subset_impl :
+    Proper (subset --> subset ==> impl) strict_subset.
+
+  Proof.
+    intros P P' P'P Q Q' QQ' [PQ n]; unfold flip in P'P. split.
+    rewrite P'P, <- QQ'. hyp. intro Q'P'. apply n. rewrite QQ', Q'P'. hyp.
+  Qed.
+
+  Global Instance strict_subset_equiv :
+    Proper (equiv ==> equiv ==> impl) strict_subset.
+
+  Proof.
+    intros P P' PP' Q Q' QQ' [PQ n]. split.
+    rewrite <- PP', <- QQ'. hyp.
+    intro Q'P'. apply n. rewrite QQ', PP'. hyp.
+  Qed.
+
+(****************************************************************************)
+(** Properties of [empty]. *)
+
+  Lemma notin_empty x : ~mem x empty.
+
+  Proof. fo. Qed.
+
+(****************************************************************************)
+(** Properties of [all]. *)
+
+  Lemma subset_all P : P [<=] all.
+
+  Proof. fo. Qed.
+
+(****************************************************************************)
+(** Properties of [add]. *)
+
+  Global Instance add_subset : Proper (eq ==> subset ==> subset) add.
+
+  Proof. intros a b ab P Q PQ. subst. fo. Qed.
+
+  Lemma subset_add a P : P [<=] add a P.
+
+  Proof. fo. Qed.
+
+  Lemma mem_add a P : mem a (add a P).
+
+  Proof. fo. Qed.
+
+  Global Instance add_equiv : Proper (eq ==> equiv ==> equiv) add.
+
+  Proof. intros a b ab P Q PQ. subst b. fo. Qed.
+
+  Lemma add_already_in a P : mem a P -> add a P [=] P.
+
+  Proof. intros a_in_P x. split; fo. subst. hyp. Qed.
+
+  Arguments add_already_in [a P] _ _.
+
+(****************************************************************************)
+(** Properties of [rem]. *)
+
+  Global Instance rem_subset : Proper (eq ==> subset ==> subset) rem.
+
+  Proof. intros a b ab P Q PQ. subst b. fo. Qed.
+
+  Global Instance rem_equiv : Proper (eq ==> equiv ==> equiv) rem.
+
+  Proof. intros a b ab P Q PQ. subst b. fo. Qed.
+
+  Lemma notin_rem a P : ~mem a (rem a P).
+
+  Proof. fo. Qed.
+
+  Lemma rem_notin a P : ~mem a P -> rem a P [=] P.
+
+  Proof. intros a_notin_P x. fo. intro e. subst. fo. Qed.
+
+  Lemma subset_rem a P : rem a P [<=] P.
+
+  Proof. fo. Qed.
+
+  Lemma strict_subset_rem a P : mem a P -> rem a P [<] P.
+
+  Proof.
+    intro aP. split. apply subset_rem. intro h. apply h in aP. revert aP.
+    apply notin_rem.
+  Qed.
+
+  Lemma add_rem_neq a b P : a <> b -> add a (rem b P) [=] rem b (add a P).
+ 
+  Proof. intro nab. split. fo. subst. hyp. fo. Qed.
+
+  Lemma rem_add_neq a b P : a <> b -> rem a (add b P) [=] add b (rem a P).
+ 
+  Proof. intro nab. split. fo. fo. subst. fo. Qed.
+
+  Lemma add_rem (eq_dec : eq_dec_type) a P : mem a P -> add a (rem a P) [=] P.
+
+  Proof. intros aP x. split. fo. subst. hyp. stac. Qed.
+
+  Arguments add_rem _ [a P] _ _.
+
+  Lemma rem_add a P : ~mem a P -> rem a (add a P) [=] P.
+
+  Proof. intros naP x. fo. intro; subst; contr. Qed.
+
+  Arguments rem_add [a P] _ _.
+
+(****************************************************************************)
+(** Properties of [union]. *)
+
+  Global Instance union_subset : Proper (subset ==> subset ==> subset) union.
+
+  Proof. fo. Qed.
+
+  Global Instance union_equiv : Proper (equiv ==> equiv ==> equiv) union.
+
+  Proof. fo. Qed.
+
+  Lemma union_com P Q : union P Q [=] union Q P.
+
+  Proof. fo. Qed.
+
+  Lemma union_assoc P Q R : union (union P Q) R [=] union P (union Q R).
+
+  Proof. fo. Qed.
+
+  Lemma subset_union_l P Q : P [<=] union P Q.
+
+  Proof. fo. Qed.
+
+  Lemma subset_union_r P Q : Q [<=] union P Q.
+
+  Proof. fo. Qed.
+
+  Lemma union_empty_l P : union empty P [=] P.
+
+  Proof. fo. Qed.
+
+  Lemma union_empty_r P : union P empty [=] P.
+
+  Proof. fo. Qed.
+
+(****************************************************************************)
+(** Properties of [diff]. *)
+
+  Global Instance diff_subset : Proper (subset ==> subset --> subset) diff.
+
+  Proof. fo. Qed.
+
+  Global Instance diff_equiv : Proper (equiv ==> equiv ==> equiv) diff.
+
+  Proof. fo. Qed.
+
+  Lemma union_diff P Q (Q_dec : forall x, {Q x}+{~Q x}) :
+    union (diff P Q) Q [=] union P Q.
+
+  Proof. split. fo. unfold union, diff, mem. destruct (Q_dec a); tauto. Qed.
+
+(****************************************************************************)
+(** Type of elements of a set. *)
+
+  Definition elts (P : set) := sig (fun x => mem x P).
+
+  Definition elt_val {P} (x : elts P) := proj1_sig x.
+
+  Coercion elt_val : elts >-> A.
+
+  Definition elts_subset P Q : P [<=] Q -> elts P -> elts Q.
+
+  Proof. intros PQ [x_val x]. ex x_val. apply PQ. hyp. Defined.
+
+  Lemma inj_elts_subset P Q (h : P [<=] Q) : injective (elts_subset h).
+
+  Proof.
+    intros [x_val x] [y_val y] e. apply sig_eq in e. apply sig_eq. hyp.
+  Qed.
+
+  Definition elts_equiv P Q : P [=] Q -> elts P -> elts Q.
+
+  Proof. intros PQ [x_val x]. apply exist with (x:=x_val). fo. Defined.
+
+  Definition elts_eq {P} : relation (elts P) :=
+    fun x y => elt_val x = elt_val y.
+
+  Instance elts_eq_Equivalence P : Equivalence (@elts_eq P).
+
+  Proof.
+    split. fo. fo.
+    intros x y z xy yz. unfold elts_eq in *. trans (elt_val y); hyp.
+  Qed.
+
+(****************************************************************************)
+(** Element belonging to a set. *)
+
+  Definition elt {P x} (h : mem x P) : elts P := @exist _ P _ h.
+
+(****************************************************************************)
+(** Fiber. *)
+
+  Definition fiber (P : set) B (f : elts P -> B) b : set :=
+    fun x => exists h : mem x P, f (elt h) = b.
+
+(****************************************************************************)
+(** Properties of [of_list]. *)
+
+  Lemma of_cons a l : of_list (a :: l) [=] add a (of_list l). 
+
+  Proof. fo. Qed.
+
+  Lemma of_remove (eq_dec : eq_dec_type) a :
+    forall l, of_list (remove eq_dec a l) [=] rem a (of_list l). 
+
+  Proof.
+    induction l; simpl. fo. destruct (eq_dec a0 a). subst. fo.
+    rewrite !of_cons, IHl, add_rem_neq, rem_add_neq; auto. refl.
+  Qed.
+
+  Lemma of_app l m : of_list (l++m) [=] union (of_list l) (of_list m).
+
+  Proof.
+    intro x. fo. destruct (in_app_or H); fo.
+    apply in_appl. hyp. apply in_appr. hyp.
+  Qed.
+
+  Lemma of_map_L P n (f : N n -> elts P) :
+    surjective f -> P [=] of_list (map (elt_val o f) (L n)).
+
+  Proof.
+    intro f_surj. set (g := elt_val o f).
+    rewrite equiv_subset2. split; intros x_val x.
+    (* P <= of_list (map g (L n)) *)
+    unfold mem, of_list. destruct (f_surj (elt x)) as [[k_val k] e].
+    apply sig_eq in e; simpl in e. subst.
+    change (In (g (N_ k)) (map g (L n))). apply in_map. apply In_L.
+    (* of_list (map g (L n)) <= P *)
+    unfold mem, of_list in x. destruct (in_map_elim x) as [k [k1 k2]].
+    subst. unfold g, comp. destruct (f k) as [y_val y]. fo.
+  Qed.
+
+End S.
+
+Arguments set: clear implicits.
+
+Infix "[<=]" := subset (at level 70).
 Infix "[=]" := equiv (at level 70).
-Infix "++" := union (right associativity, at level 60).
-Infix "::" := add (at level 60, right associativity).
+Infix "[<]" := strict_subset (at level 70).
 
 (***********************************************************************)
-(** Inclusion. *)
+(** Compatibility with [inclusion] and [same_rel]. *)
 
-Instance incl_preorder A : PreOrder (@incl A).
-
-Proof. fo. Qed.
-
-Lemma incl_appl : forall X (A B : set X), A [= A ++ B.
-
-Proof. fo. Qed.
-
-Lemma incl_appr : forall X (A B : set X), A [= B ++ A.
-
-Proof. fo. Qed.
-
-(***********************************************************************)
-(** Equality. *)
-
-Lemma equiv_inter_transp : forall X, @equiv X == inter_transp (@incl X).
-
-Proof. fo. Qed.
-
-Lemma equiv_elim : forall X (A B : set X), A [=] B <-> A [= B /\ B [= A.
-
-Proof. fo. Qed.
-
-Instance incl_equiv1 A1 B (f : set A1 -> relation B) :
-  Proper (incl ==> inclusion) f -> Proper (equiv ==> same_rel) f.
+Instance subset_equiv1 A1 B (f : set A1 -> relation B) :
+  Proper (subset ==> inclusion) f -> Proper (equiv ==> same_rel) f.
 
 Proof. intros hf s1 s1'. rewrite equiv_elim. fo. Qed.
 
-Instance incl_equiv2 A1 A2 B (f : set A1 -> set A2 -> relation B) :
-  Proper (incl ==> incl ==> inclusion) f ->
+Instance subset_equiv2 A1 A2 B (f : set A1 -> set A2 -> relation B) :
+  Proper (subset ==> subset ==> inclusion) f ->
   Proper (equiv ==> equiv ==> same_rel) f.
 
 Proof.
@@ -81,37 +383,7 @@ Proof.
 Qed.
 
 (***********************************************************************)
-(** Union. *)
-
-Instance union_incl A : Proper (incl ==> incl ==> incl) (@union A).
-
-Proof. fo. Qed.
-
-Instance union_equiv A : Proper (equiv ==> equiv ==> equiv) (@union A).
-
-Proof. fo. Qed.
-
-Lemma empty_union_l : forall X (A : set X), empty ++ A [=] A.
-
-Proof. fo. Qed.
-
-Lemma empty_union_r : forall X (A : set X), A ++ empty [=] A.
-
-Proof. fo. Qed.
-
-(***********************************************************************)
-(** Add. *)
-
-Instance add_incl A : Proper (eq ==> incl ==> incl) (@add A).
-
-Proof. intros x x' xx'. subst x'. fo. Qed.
-
-Instance add_equiv A : Proper (eq ==> equiv ==> equiv) (@add A).
-
-Proof. intros x x' xx'. subst x'. fo. Qed.
-
-(***********************************************************************)
-(** Image by a function. *)
+(** Image of a set by a function. *)
 
 Section image.
 
@@ -119,20 +391,20 @@ Section image.
 
   Definition image (A : set X) : set Y := fun y => exists x, A x /\ y = f x.
 
-  Lemma image_singleton x : image (singleton x) [=] singleton (f x).
-
-  Proof.
-    intro y. split.
-    intros [a [h1 h2]]. unfold singleton in *. subst. refl.
-    unfold singleton. intro h. exists x. auto.
-  Qed.
-
-  Lemma image_union A B : image (A ++ B) [=] image A ++ image B.
+  Lemma image_empty : image empty [=] empty.
 
   Proof. fo. Qed.
 
-  Lemma image_add x A : image (x :: A) [=] f x :: image A.
+  Lemma image_add a A : image (add a A) [=] add (f a) (image A).
 
-  Proof. unfold add. rewrite image_union, image_singleton. refl. Qed.
+  Proof. intro x. split. fo. subst. fo. fo. Qed.
+
+  Lemma image_singleton x : image (singleton x) [=] singleton (f x).
+
+  Proof. unfold singleton. rewrite image_add, image_empty. refl. Qed.
+
+  Lemma image_union A B : image (union A B) [=] union (image A) (image B).
+
+  Proof. fo. Qed.
 
 End image.
